initial comit with some progress

WebAssembly/Wasm_Instantiation_Properties.thy
@@ -1,4 +1,4 @@
-theory Wasm_Instantiation_Properties imports Wasm_Instantiation begin
+theory Wasm_Instantiation_Properties imports Wasm_Instantiation Wasm_Properties begin
 
 lemma list_all_ex_list_all2:
   assumes "\<And>i. i < length xs \<Longrightarrow> \<exists>y. P (xs!i) y"
@@ -15,6 +15,248 @@ proof (induction xs)
     by blast
 qed auto
 
+
+lemma store_extension_intros_with_refl: 
+  assumes "funcs s = funcs s' \<or> (\<exists> fs. funcs s @ fs = funcs s')" 
+  "tabs s = tabs s' \<or> (\<exists> t1 t2. t1 @ t2 = tabs s' \<and> list_all2 tab_extension (tabs s) t1)"
+  "mems s = mems s' \<or> (\<exists> m1 m2. m1 @ m2 = mems s' \<and> list_all2 mem_extension (mems s) m1)" 
+  "globs s = globs s' \<or> (\<exists> g1 g2. g1 @ g2 = globs s' \<and> list_all2 global_extension (globs s) g1)" 
+  shows "store_extension s s'"
+proof -         
+  have funcs:"\<exists> fs. funcs s @ fs = funcs s'" using assms(1) by auto
+
+  have tabs: "\<exists> t1 t2. t1 @ t2 = tabs s' \<and> list_all2 tab_extension (tabs s) t1" 
+    using assms(2) tab_extension_refl list_all2_refl
+    by (metis append_Nil2) 
+
+  have mems: "\<exists> m1 m2. m1 @ m2 = mems s' \<and> list_all2 mem_extension (mems s) m1" 
+    using assms(3) mem_extension_refl list_all2_refl
+    by (metis append_Nil2) 
+
+  have globs: "\<exists> g1 g2. g1 @ g2 = globs s' \<and> list_all2 global_extension (globs s) g1"  
+    using assms(4) global_extension_refl list_all2_refl
+    by (metis append_Nil2) 
+  
+  show ?thesis using funcs mems tabs globs unfolding store_extension.simps
+    by (metis (full_types) unit.exhaust s.surjective) 
+qed
+
+lemma init_tab_form:
+  assumes "s' = init_tab s inst e_ind e" 
+  shows "list_all2 tab_extension (tabs s) (tabs s')" 
+        "\<exists>tabs'. s' = s\<lparr>tabs := tabs'\<rparr>"
+proof -
+  obtain t_ind tab_e max e_pay tab'_e where init_tab_is:
+    "t_ind = ((inst.tabs inst)!(e_tab e))" 
+    "(tab_e,max) = (tabs s)!t_ind" 
+    "e_pay = map (\<lambda>i. Some ((inst.funcs inst)!i)) (e_init e)"
+    "tab'_e = ((take e_ind tab_e) @ e_pay @ (drop (e_ind + length e_pay) tab_e))" 
+    by (metis prod.exhaust)
+
+  then have "init_tab s inst e_ind e = s\<lparr>tabs := (tabs s)[t_ind := (tab'_e,max)]\<rparr>" 
+    unfolding init_tab_def by(fastforce simp add: Let_def split: prod.splits)
+  then have 1:"s' = s\<lparr>tabs := (tabs s)[t_ind := (tab'_e,max)]\<rparr>" using assms by auto 
+
+  have "length tab_e \<le> length tab'_e" using init_tab_is
+    by simp 
+  then have "tab_extension ((tabs s)!t_ind) (tab'_e, max)" 
+    unfolding tab_extension_def using init_tab_is
+    by (metis fst_conv snd_conv) 
+  then show "list_all2 tab_extension (tabs s) (tabs s')"  
+    using init_tab_is  tab_extension_refl unfolding 1 list_all2_conv_all_nth  
+    by (simp, metis nth_list_update_eq nth_list_update_neq)
+
+  show "\<exists>tabs'. s' = s\<lparr>tabs := tabs'\<rparr>" unfolding assms init_tab_def
+    by(simp add: Let_def exI split:prod.splits)
+qed
+
+lemma tab_extension_trans:"tab_extension a b \<Longrightarrow> tab_extension b c \<Longrightarrow> tab_extension a c" 
+  unfolding tab_extension_def by auto
+
+
+lemma init_tabs_form:
+  assumes "s' = init_tabs s inst e_inds es" 
+  shows "list_all2 tab_extension (tabs s) (tabs s')" 
+        "\<exists>tabs'. s' = s\<lparr>tabs := tabs'\<rparr>"
+proof -
+  {
+    fix a
+    have "s' = foldl (\<lambda>s' (e_ind,e). init_tab s' inst e_ind e) s a \<Longrightarrow> 
+          list_all2 tab_extension (tabs s) (tabs s') \<and> (\<exists>tabs'. s' = s\<lparr>tabs := tabs'\<rparr>)"
+    proof (induction a arbitrary:s)
+      case Nil
+      show ?case using Nil exI[where x="tabs s"] unfolding foldl_Nil 
+        by(simp add: list_all2_refl tab_extension_refl)  
+    next
+      case (Cons a1 a2)
+      define s_mid where "s_mid = init_tab s inst (fst a1) (snd a1)" 
+      then have 1:"s' = foldl (\<lambda>s' (e_ind,e). init_tab s' inst e_ind e) s_mid a2" 
+        using Cons foldl_Cons
+        by(simp add: case_prod_beta')
+
+      note ind_assms = init_tab_form[OF s_mid_def] Cons(1)[OF 1]
+
+      have "list_all2 tab_extension (tabs s) (tabs s')" using ind_assms
+        list_all2_trans tab_extension_trans
+        by blast
+      moreover have "\<exists>tabs'. s' = s\<lparr>tabs := tabs'\<rparr>" using ind_assms
+        by auto
+      ultimately show ?case by auto
+    qed 
+  }
+  note helper = this
+  show "list_all2 tab_extension (tabs s) (tabs s')" using helper assms unfolding init_tabs_def
+    by presburger 
+  show "\<exists>tabs'. s' = s\<lparr>tabs := tabs'\<rparr>" using helper assms unfolding init_tabs_def
+    by presburger
+qed
+
+lemma init_tabs_preserve_funcs:
+  assumes "s' = init_tabs s inst e_inds es" 
+  shows "funcs s' = funcs s"
+  using init_tabs_form(2)[OF assms]
+  by auto
+
+
+lemma init_tabs_preserve_store_extension: 
+  assumes "s' = init_tabs s inst e_inds es" 
+  shows "store_extension s s'"
+  using init_tabs_form[OF assms] store_extension_intros_with_refl
+  by (metis append_Nil2 s.ext_inject s.surjective s.update_convs(2))   
+
+lemma init_mem_form:
+  assumes "s' = init_mem s inst d_ind d" 
+  shows "list_all2 mem_extension (mems s) (mems s')" 
+        "\<exists>mems'. s' = s\<lparr>mems := mems'\<rparr>"
+proof -
+  obtain m_ind mem mem' where init_mem_is: "m_ind = ((inst.mems inst)!(d_data d))"
+                               "mem = (mems s)!m_ind"
+                               "mem' = write_bytes mem d_ind (d_init d)"
+                               "s' =s\<lparr>mems := (mems s)[m_ind := mem']\<rparr>" 
+    using assms unfolding init_mem_def Let_def by auto 
+
+  have "mem_size mem \<le> mem_size mem'" using init_mem_is
+    by (simp add: div_le_mono mem_length_def mem_rep_length.rep_eq 
+       mem_rep_write_bytes.rep_eq mem_size_def write_bytes_def)
+     (* sledgehammer :P *) 
+
+  moreover have "mem_max mem = mem_max mem'" using init_mem_is
+    by (simp add: mem_max_def write_bytes_def) 
+
+  ultimately have "mem_extension mem mem'" 
+    unfolding mem_extension_def by auto
+
+  then show "list_all2 mem_extension (mems s) (mems s')"  
+    using init_mem_is mem_extension_refl unfolding init_mem_is(4) list_all2_conv_all_nth  
+    by (simp, metis nth_list_update_eq nth_list_update_neq)
+
+  show "\<exists>mems'. s' = s\<lparr>mems := mems'\<rparr>" unfolding assms init_mem_def
+    by(simp add: Let_def exI split:prod.splits)
+qed
+
+
+lemma mem_extension_trans:"mem_extension a b \<Longrightarrow> mem_extension b c \<Longrightarrow> mem_extension a c" 
+  unfolding mem_extension_def by auto
+
+lemma init_mems_form:
+  assumes "s' = init_mems s inst d_inds ds" 
+  shows "list_all2 mem_extension (mems s) (mems s')" 
+        "\<exists>mems'. s' = s\<lparr>mems := mems'\<rparr>"
+proof -
+  {
+    fix a
+    have "s' = foldl (\<lambda>s' (d_ind,d). init_mem s' inst d_ind d) s a \<Longrightarrow> 
+          list_all2 mem_extension (mems s) (mems s') \<and> (\<exists>mems'. s' = s\<lparr>mems := mems'\<rparr>)"
+    proof (induction a arbitrary:s)
+      case Nil
+      show ?case using Nil exI[where x="mems s"] unfolding foldl_Nil 
+        by(simp add: list_all2_refl mem_extension_refl)  
+    next
+      case (Cons a1 a2)
+      define s_mid where "s_mid = init_mem s inst (fst a1) (snd a1)" 
+      then have 1:"s' = foldl (\<lambda>s' (d_ind,d). init_mem s' inst d_ind d) s_mid a2" 
+        using Cons foldl_Cons
+        by(simp add: case_prod_beta')
+
+      note ind_assms = init_mem_form[OF s_mid_def] Cons(1)[OF 1]
+
+      have "list_all2 mem_extension (mems s) (mems s')" using ind_assms
+        list_all2_trans mem_extension_trans
+        by blast
+      moreover have "\<exists>mems'. s' = s\<lparr>mems := mems'\<rparr>" using ind_assms
+        by auto
+      ultimately show ?case by auto
+    qed 
+  }
+  note helper = this
+  show "list_all2 mem_extension (mems s) (mems s')" using helper assms unfolding init_mems_def
+    by presburger 
+  show "\<exists>mems'. s' = s\<lparr>mems := mems'\<rparr>" using helper assms unfolding init_mems_def
+    by presburger
+qed
+
+lemma init_mems_preserve_funcs:
+  assumes "s' = init_mems s inst d_inds ds" 
+  shows "funcs s' = funcs s"
+  using init_mems_form(2)[OF assms]
+  by auto
+
+lemma init_mems_preserve_store_extension: 
+  assumes "s' = init_mems s inst d_inds ds" 
+  shows "store_extension s s'"
+  using init_mems_form[OF assms] store_extension_intros_with_refl
+  by (metis append_Nil2 s.ext_inject s.surjective s.update_convs(3))   
+
+lemma alloc_module_preserve_store_extension:
+  assumes "alloc_module s m imps gvs (s',inst,exps)" 
+  shows "store_extension s s'"
+  using alloc_module_ext_arb[OF assms] 
+  store_extension_intros_with_refl list_all2_refl tab_extension_refl mem_extension_refl global_extension_refl
+  by metis
+
+lemma alloc_module_funcs_only_alloc_func:
+  assumes "alloc_module s m imps gvs (s',inst,exps)"
+    "alloc_funcs s (m_funcs m) inst = (s1,i_fs)"
+  shows "funcs s' = funcs s1" 
+  using assms alloc_tabs_range alloc_mems_range alloc_globs_range 
+  unfolding alloc_module.simps 
+  by force 
+
+lemma list_all2_in_set:
+  assumes "x\<in>set xs" "list_all2 f xs ys" 
+  shows "\<exists>y. f x y" 
+  using assms 
+  by (smt (verit, best) list_all2_conv_all_nth mem_Collect_eq set_conv_nth)
+
+
+
+definition alloc_func_fs :: "module_func \<Rightarrow> inst \<Rightarrow> cl" where
+  "alloc_func_fs m_f inst =
+     (case m_f of (i_t, loc_ts, b_es) \<Rightarrow>
+        Func_native inst ((types inst)!i_t) loc_ts b_es)"
+
+lemma alloc_func_equiv:"fst (alloc_func s m_f i) = s\<lparr>funcs := funcs s @ [alloc_func_fs m_f i]\<rparr>"
+  using alloc_func_def alloc_func_fs_def by(simp split:prod.splits)
+
+abbreviation "alloc_funcs_fs m_fs i \<equiv> map (\<lambda>m_f. alloc_func_fs m_f i) m_fs"
+
+lemma alloc_funcs_equiv:"fst (alloc_funcs s m_fs i) = s\<lparr>funcs := funcs s @ alloc_funcs_fs m_fs i\<rparr>"
+proof(induct m_fs arbitrary: s)
+  case Nil
+  then show ?case by auto 
+next
+  case (Cons a m_fs)
+  have "fst (alloc_funcs s (a # m_fs) i) = fst (alloc_funcs (fst (alloc_func s a i)) m_fs i)"
+    using alloc_Xs.simps(2) by(simp split:prod.splits)
+
+  also have "... = fst (alloc_funcs (s\<lparr>funcs := funcs s @ [alloc_func_fs a i]\<rparr>) m_fs i)" 
+    using alloc_func_equiv by simp
+
+  also have "... = s\<lparr>funcs := funcs s @ alloc_funcs_fs (a#m_fs) i\<rparr> " 
+    using Cons by auto
+  finally show ?case by auto
+qed
+   
 theorem instantiation_sound:
   assumes "store_typing s"
           "(instantiate s m v_imps ((s', inst, v_exps), start))"
@@ -23,11 +265,98 @@ theorem instantiation_sound:
         "\<exists>tes. list_all2 (\<lambda>v_exp te. external_typing s' (E_desc v_exp) te) v_exps tes"
         "pred_option (\<lambda>i. i < length (s.funcs s')) start"
 proof -
+  obtain s1 s2 t_imps t_exps g_inits f e_offs d_offs where 
+    "module_typing m t_imps t_exps"
+    "list_all2 (external_typing s) v_imps t_imps"
+    and s_alloc_module:"alloc_module s m v_imps g_inits (s1, inst, v_exps)"
+    and "f = \<lparr> f_locs = [], f_inst = inst \<rparr>"
+    "list_all2 (\<lambda>g v. reduce_trans (s1,f,$*(g_init g)) (s1,f,[$C v])) (m_globs m) g_inits"
+    "list_all2 (\<lambda>e c. reduce_trans (s1,f,$*(e_off e)) (s1,f,[$C ConstInt32 c])) (m_elem m) e_offs"
+    "list_all2 (\<lambda>d c. reduce_trans (s1,f,$*(d_off d)) (s1,f,[$C ConstInt32 c])) (m_data m) d_offs"
+    "list_all2 (\<lambda>e_off e. ((nat_of_int e_off) + (length (e_init e))) \<le> length (fst ((tabs s1)!((inst.tabs inst)!(e_tab e))))) e_offs (m_elem m)"
+    "list_all2 (\<lambda>d_off d. ((nat_of_int d_off) + (length (d_init d))) \<le> mem_length ((mems s1)!((inst.mems inst)!(d_data d)))) d_offs (m_data m)"
+    "map_option (\<lambda>i_s. ((inst.funcs inst)!i_s)) (m_start m) = start"
+    and s_init_tabs:"init_tabs s1 inst (map nat_of_int e_offs) (m_elem m) = s2"
+    and s_init_mems:"init_mems s2 inst (map nat_of_int d_offs) (m_data m) = s'" 
+    using assms(2) instantiate.simps by auto
+
+  have "store_extension s s1" using alloc_module_preserve_store_extension s_alloc_module by auto
+  have "store_extension s1 s2" using init_tabs_preserve_store_extension s_init_tabs by auto 
+  have "store_extension s2 s'" using init_mems_preserve_store_extension s_init_mems by auto 
+
+  obtain \<C> fts els ds i_opt where c_is:"list_all2 (module_func_typing \<C>) (m_funcs m) fts"
+    "list_all (module_elem_typing \<C>) els"
+    "list_all (module_data_typing \<C>) ds"
+    "pred_option (module_start_typing \<C>) i_opt"
+    using \<open>module_typing m t_imps t_exps\<close> module_typing.simps
+    by auto 
+
+  have "inst_typing s1 inst \<C>" sorry
 
   show "store_typing s'"
   proof -
-    have 1:"list_all (\<lambda>cl. \<exists>tf. cl_typing s' cl tf) (funcs s')"
-      sorry
+    have 1:"list_all (\<lambda>cl. \<exists>tf. cl_typing s' cl tf) (funcs s')" 
+    proof -
+      have s1_cl_typing:"list_all (\<lambda>cl. \<exists>tf. cl_typing s1 cl tf) (funcs s1)" 
+      proof - 
+        obtain fs where "funcs s1 = funcs s @ fs" using alloc_module_ext_arb[OF s_alloc_module]
+          by metis
+
+        have "list_all (\<lambda>cl. \<exists>tf. cl_typing s1 cl tf) (funcs s)" 
+          using cl_typing_store_extension_inv[OF \<open>store_extension s s1\<close>] store_typing.simps assms(1)
+          by (smt (verit, ccfv_threshold) list_all_length) 
+        moreover have "list_all (\<lambda>cl. \<exists>tf. cl_typing s1 cl tf) fs" 
+        proof -
+          {
+            fix f
+            assume "f\<in>set fs" 
+
+            define s_mid where s_mid_def:"s_mid = fst (alloc_funcs s (m_funcs m) inst)"
+            then have "funcs s1 = funcs s_mid" 
+              using alloc_module_funcs_only_alloc_func[OF s_alloc_module]
+              by (metis eq_fst_iff) 
+            then have "funcs s_mid = funcs s @ fs" using \<open>funcs s1 = funcs s @ fs\<close> by auto
+            then have 0:"alloc_funcs_fs (m_funcs m) inst = fs" 
+              using alloc_funcs_equiv s_mid_def by auto
+            
+            obtain i_t loc_ts b_es where 1:
+              "f = Func_native inst ((types inst)!i_t) loc_ts b_es"  
+              "(i_t, loc_ts, b_es) \<in> set (m_funcs m)"
+              using 0 \<open>f\<in> set fs\<close> unfolding alloc_func_fs_def by auto
+
+            obtain tn tm where 2:
+              "i_t < length (types_t \<C>)"
+              "(types_t \<C>)!i_t = (tn _> tm)"
+              "\<C>\<lparr>local := tn @ loc_ts, label := ([tm] @ (label \<C>)), return := Some tm\<rparr> \<turnstile> b_es : ([] _> tm)"
+              using list_all2_in_set[OF 1(2) c_is(1)]
+              unfolding module_func_typing.simps by auto 
+
+            have 3:"(types inst)!i_t = (types_t \<C>)!i_t"
+              using store_typing_imp_types_eq[OF \<open>inst_typing s1 inst \<C>\<close> 2(1)] by auto
+
+            have "cl_typing s1 f (tn _> tm)" 
+              using 1(1) 2 3 
+              cl_typing.intros(1)[OF \<open>inst_typing s1 inst \<C>\<close>]
+              by presburger 
+            then have "\<exists>tf. cl_typing s1 f tf" by auto
+          }
+          then show ?thesis by (simp add: list_all_iff) 
+        qed
+        ultimately show ?thesis using \<open>funcs s1 = funcs s @ fs\<close> by auto
+      qed 
+      have s2_cl_typing:"list_all (\<lambda>cl. \<exists>tf. cl_typing s2 cl tf) (funcs s2)"
+      proof -
+        have "funcs s1 = funcs s2" using init_tabs_preserve_funcs s_init_tabs by auto
+        then show ?thesis using cl_typing_store_extension_inv[OF \<open>store_extension s1 s2\<close>] s1_cl_typing 
+          by (smt (verit, best) list_all_length)
+      qed  
+      show  "list_all (\<lambda>cl. \<exists>tf. cl_typing s' cl tf) (funcs s')" 
+      proof -
+        have "funcs s2 = funcs s'" using init_mems_preserve_funcs s_init_mems by auto
+        then show ?thesis using cl_typing_store_extension_inv[OF \<open>store_extension s2 s'\<close>] s2_cl_typing 
+          by (smt (verit, best) list_all_length)
+      qed 
+    qed
     have 2:"list_all (tab_agree s') (tabs s')"
       sorry
     have 3:"list_all mem_agree (mems s')"
@@ -39,17 +368,13 @@ proof -
 
   show "\<exists>\<C>. inst_typing s' inst \<C>"
   proof -
-    have 1:"\<exists>tfs. list_all2 (funci_agree (funcs s')) (inst.funcs inst) tfs"
-      sorry
-    have 2:"\<exists>tgs. list_all2 (globi_agree (globs s')) (inst.globs inst) tgs"
-      sorry
-    have 3:"\<exists>tabs_t. list_all2 (tabi_agree (tabs s')) (inst.tabs inst) tabs_t"
-      sorry
-    have 4:"\<exists>mems_t. list_all2 (memi_agree (mems s')) (inst.mems inst) mems_t"
-      sorry
-    show ?thesis
-      using 1 2 3 4 inst_typing.intros
-      by (metis (full_types) inst.surjective unit.exhaust)
+    have "inst_typing s2 inst \<C>" 
+      using inst_typing_store_extension_inv[OF \<open>inst_typing s1 inst \<C>\<close>  \<open>store_extension s1 s2\<close>]
+      by simp 
+    then have "inst_typing s' inst \<C>" 
+      using inst_typing_store_extension_inv  \<open>store_extension s2 s'\<close>
+      by simp
+    then show ?thesis by auto
   qed
 
   show "\<exists>tes. list_all2 (\<lambda>v_exp te. external_typing s' (E_desc v_exp) te) v_exps tes"
